Finish all but one obligation
The remaining one is false.  We have finally reached the point where
we need to minimize the parse tree, rather than taking the top of it.
To do this, I think it suffices to pass around a shallowly-minimal
tree, where, whenever we chop off a name, we recurse down to be sure
we don't see that name until we reset the valid list.

src/Parsers/DependentlyTypedMinimalOfParse.v
@@ -15,11 +15,11 @@ Section recursive_descent_parser.
           (String : string_like CharType)
           (G : grammar CharType).
   Context {premethods : parser_computational_predataT}.
-  Context (remove_name_1
+  Context (remove_nonterminal_name_1
            : forall ls ps ps',
                is_valid_nonterminal_name (remove_nonterminal_name ls ps) ps' = true
                -> is_valid_nonterminal_name ls ps' = true)
-          (remove_name_2
+          (remove_nonterminal_name_2
            : forall ls ps ps',
                is_valid_nonterminal_name (remove_nonterminal_name ls ps) ps' = false
                <-> is_valid_nonterminal_name ls ps' = false \/ ps = ps').
@@ -201,6 +201,10 @@ Section recursive_descent_parser.
                               -> sub_names_listT is_valid_nonterminal_name valid initial_nonterminal_names_data
                               -> T.
 
+          Let alt := False (*{ nonterminal_name : string
+                     | is_valid_nonterminal_name initial_nonterminal_names_data nonterminal_name = true
+                       /\ is_valid_nonterminal_name valid nonterminal_name = false }*).
+
           Section T_nonterminal_name.
             Context (name : string) (str : StringWithSplitState String (split_stateT (include_nonterminal_name _ name))).
             Let ret := mp_parse_nonterminal_name str0 valid str name.
@@ -211,7 +215,7 @@ Section recursive_descent_parser.
             Definition T_nonterminal_name_failure : Type
               := prefix str match state_val str with
                               | None => ret -> False
-                              | Some p => False
+                              | Some p => alt
                             end.
           End T_nonterminal_name.
 
@@ -225,7 +229,7 @@ Section recursive_descent_parser.
             Definition T_item_failure : Type
               := prefix str match state_val str with
                               | None => ret -> False
-                              | Some p => False
+                              | Some p => alt
                             end.
           End T_item.
 
@@ -239,7 +243,7 @@ Section recursive_descent_parser.
             Definition T_production_failure : Type
               := prefix str match state_val str with
                               | None => ret -> False
-                              | Some p => False
+                              | Some p => alt
                             end.
           End T_production.
 
@@ -254,7 +258,7 @@ Section recursive_descent_parser.
             Definition T_productions_failure : Type
               := prefix str match state_val str with
                               | None => ret -> False
-                              | Some p => False
+                              | Some p => alt
                             end.
           End T_productions.
         End types.
@@ -364,20 +368,35 @@ Section recursive_descent_parser.
         Hint Constructors minimal_parse_of minimal_parse_of_name minimal_parse_of_production minimal_parse_of_item unit prod unit : minimal_instance_db.
         Hint Unfold T_item_success T_item_failure T_production_success T_production_failure T_productions_success T_productions_failure T_nonterminal_name_success T_nonterminal_name_failure
              DependentlyTyped.T_item_success DependentlyTyped.T_item_failure DependentlyTyped.T_production_success DependentlyTyped.T_production_failure DependentlyTyped.T_productions_success DependentlyTyped.T_productions_failure DependentlyTyped.T_nonterminal_name_success DependentlyTyped.T_nonterminal_name_failure
-             p_parse_production mp_parse_production p_parse mp_parse p_parse_item mp_parse_item p_parse_nonterminal_name mp_parse_nonterminal_name string_val : minimal_instance_db.
+             p_parse_production p_parse p_parse_item p_parse_nonterminal_name
+             mp_parse_production mp_parse mp_parse_item mp_parse_nonterminal_name : minimal_instance_db.
 
         Local Ltac t''0 :=
-          first [ intro
-                | progress subst_body
+          first [ progress cbv zeta
+                | intro
+                (*| progress subst_body*)
+                | let H := (match goal with
+                              | [ H : StringWithSplitState _ _ |- _ ] => constr:H
+                              | [ H : ?T |- _ ] => match eval hnf in T with
+                                                     | StringWithSplitState _ _
+                                                       => constr:H
+                                                   end
+                            end) in
+                  let s := fresh "s" in
+                  let st := fresh "st" in
+                  destruct H as [s st];
+                    change (StringLike.Core.string_val {| string_val := s |}) with s in *;
+                    change (StringLike.Core.state_val {| state_val := st |}) with st in *;
+                    simpl
                 | match goal with
-                    | [ H : StringWithSplitState _ _ |- _ ] => destruct H; simpl
-                    | [ H : ?T |- _ ] => match eval hnf in T with
-                                           | StringWithSplitState _ _ => destruct H; simpl
-                                         end
                     | [ H : option _ |- _ ] => destruct H; simpl
                     | [ H : ?T |- _ ] => match eval hnf in T with
                                            | option _ => destruct H; simpl
                                          end
+                  end
+                | match goal with
+                    | [ H : appcontext[StringLike.Core.string_val {| string_val := ?s |}] |- _ ] => change (StringLike.Core.string_val {| string_val := s |}) with s in *
+                    | [ H : appcontext[StringLike.Core.state_val {| state_val := ?s |}] |- _ ] => change (StringLike.Core.state_val {| state_val := s |}) with s in *
                   end ].
 
         Local Ltac t'' :=
@@ -409,8 +428,11 @@ Section recursive_descent_parser.
             | [ H : sub_names_listT _ ?x ?y -> _ |- _ ] => specialize (H (reflexivity _))
             | [ H : sub_names_listT _ _ _, H' : sub_names_listT _ _ _ -> _ |- _ ]
               => specialize (fun arg => H' (sub_names_listT_remove_2 _ arg _ H))
-            (*| _ => progress hnf in * *)
+            | [ H : context[map _ nil] |- _ ] => progress simpl in H
+            | [ H : context[map _ (_::_)] |- _ ] => progress simpl in H
+            | [ H : appcontext[split_string_for_production _ _ {| state_val := Some _ |} ] |- _ ] => progress simpl in H
             | _ => progress autounfold with minimal_instance_db in *
+            (*| _ => progress hnf in * *)
             | [ H : ?T |- _ ] => match head T with
                                    | match _ with _ => _ end => progress hnf in H
                                  end
@@ -429,9 +451,13 @@ Section recursive_descent_parser.
                 |- @sigT ?A _ ]
               => exists (MinParseTail _ x : A); assumption
             | [ H : sigT _ |- _ ] => destruct H
+            | [ H : sig _ |- _ ] => destruct H
             | [ H : prod _ _ |- _ ] => destruct H
             | [ H : and _ _ |- _ ] => destruct H
             | [ H : (_, _) = (_, _) |- _ ] => apply path_prod' in H
+            | [ H : ?T |- _ ] => match eval hnf in T with
+                                   | (_ * _)%type => destruct H
+                                 end
             | _ => progress subst
             | _ => progress simpl
             | [ H : _ = _ |- _ ] => progress simpl in H (* work around [simpl in *] causing ~everything, even [admit], to error with "Anomaly: Cannot take the successor of a non variable universe:
@@ -443,8 +469,9 @@ Please report." *)
               end
             | [ H : (_ =s _) = true |- _ ] => apply bool_eq_correct in H
             | [ H : is_true (_ =s _) |- _ ] => apply bool_eq_correct in H
-            | [ H : parse_of_item _ _ ?s (Terminal ?ch) |- _ ] => atomic s; inversion H
-            | [ H : parse_of_production _ _ ?s []  |- _ ] => atomic s; inversion H
+            | [ H : parse_of_item _ _ _ (NonTerminal _ _) |- _ ] => (* work around 4035 *) let H' := fresh in rename H into H'; dependent destruction H'
+            | [ H : parse_of_item _ _ _ (Terminal _) |- _ ] => (* work around 4035 *) let H' := fresh in rename H into H'; dependent destruction H'
+            | [ H : parse_of_production _ _ _ [] |- _ ] => (* work around 4035 *) let H' := fresh in rename H into H'; dependent destruction H'
             | [ H : ?A -> ?B, H' : ?A |- _ ] => specialize (H H')
             | [ H : ?A -> False |- _ ] => let A' := (eval hnf in A) in progress change (A' -> False) in H
             | _ => progress trivial
@@ -467,7 +494,8 @@ Please report." *)
           first [ t''
                 (*| congruence*)
                 | match goal with H : true = false |- _ => exfalso; clear -H; congruence end
-                | omega
+                | match goal with H : ?x = false, H' : ?x = true |- _ => exfalso; clear -H H'; abstract congruence end
+                | abstract omega
                 | match goal with H : (?x =s ?x) = false |- _ => erewrite (proj2 (bool_eq_correct _ _ _)) in H by reflexivity end
                 | match goal with H : _ -> False |- False => apply H end;
                   abstract (repeat t'') ].
@@ -525,6 +553,22 @@ Please report." *)
         Let H_prod_splitT' str0 valid it its str st
           := split_string_lift_T str0 valid it its {| string_val := str ; state_val := st |} (split_string_for_production it its {| string_val := str ; state_val := st |}).
 
+        Lemma H_prod_split_helper str0 valid it its str st
+        : @H_prod_splitT' str0 valid it its str (Some st).
+        Proof.
+          subst_body; simpl in *.
+          intros ? H.
+          simpl in H.
+          destruct_head prod.
+          destruct_head sum;
+            destruct_head prod;
+            unfold T_item_failure, T_production_failure in *;
+            simpl in *.
+          { repeat t''. }
+          { repeat t''. }
+          { repeat t''. }
+        Defined.
+
         Start Profiling.
         Time Global Program Instance minimal_parser_dependent_types_extra_data
              (H_prod_split' : forall str0 valid it its str, @H_prod_splitT' str0 valid it its str None)
@@ -536,14 +580,180 @@ Please report." *)
                      | {| string_val := str' ; state_val := st' |}
                        => match st' with
                             | None => @H_prod_split' str0 valid it its str'
-                            | Some st => _
+                            | Some st => @H_prod_split_helper str0 valid it its str' st
                           end
                    end |}.
         Obligation 12. t. Defined.
         Obligation 13. t. Defined.
         Obligation 14. t. Defined.
-        Obligation 15. t. Defined.
+        Obligation 11. t. Defined.
+        Obligation 1. t. Defined.
+        Obligation 2. t. Defined.
+        Obligation 3. t. Defined.
+        Obligation 4. t. Defined.
+        Obligation 5. t. Defined.
+        Obligation 6. t. Defined.
+        Obligation 7. t. Defined.
+        Obligation 8. t. Defined.
+        Obligation 9. t. Defined.
+        Obligation 10. t. Defined.
+        Obligation 15.
+        simpl.
+        intros.
+        assert (str = str0 :> String).
+        { destruct_head @str_le.
+          { exfalso; eauto with nocore. }
+          { assumption. } }
+        subst.
+        clear H H0.
+        hnf.
+        repeat t''0; [ | solve [ t ] ].
+        clear H.
+        hnf in p.
+        destruct p.
+        dependent destruction x.
+        destruct f.
+
+        hnf in p0.
+
+
+        do 10 t''.
+        t''.
+        t''.
+        t''.
+        t''.
+        t''.
+        t''.
+        destruct_head prod.
+        destruct_head sum; repeat t''.
+        t''.
+        match goal with
+        end.
+        simpl split_string_for_production in *.
+        t''.
+        t''.
+        simpl in X.
+        destruct_head prod.
+        destruct_head sum.
+        repeat t''.
+        repeat t''.
+        repeat t''.
+simpl in *.
+        do 10 (simpl in *; t'').
+        t''.
+        t''.
+        t''.
+        t''.
+        t''.
+        t''.
+        t''; simpl in *.
+        t''; simpl in *.
+        t''; simpl in *.
+        t''; simpl in *.
+        t''; simpl in *.
+        t''; simpl in *.
+        t''; simpl in *.
+        t''; simpl in *.
+        simpl in X.
+        t''.
+        t''.
+        t''.
+        t''.
+        t''.
+        t''.
+        t''.
+        t''.
+        t''.
+        t''.
+        t''.
+        t''.
+        t''.
+
+        t''.
+        simpl in s.
+t. Defined.
+        Obligation 16. t. Defined.
+        Next Obligation. t. Defined.
+        Next Obligation. t. Defined.
+        Next Obligation. t. Defined.
+        Next Obligation. t. Defined.
+        Next Obligation. t. Defined.
+        Next Obligation. t. Defined.
+        Next Obligation. t. Defined.
+        Next Obligation. t. Defined.
+        Next Obligation. t. Defined.
+        Next Obligation. t. Defined.
+        Next Obligation. simpl.
+                        do 5 t''.
+                        do 5 t''.
+                        do 5 t''.
+                        t''.
+                        t''.
+                        t''.
+                        t''.
+                        t''.
+                        t''.
+                        t''.
+                        t''.
+                        t''.
+                        match goal with
+                        end.
+                        t''.
+                        do 5 t''.
+                        do 5 t''.
+                        do 5 t''.
+                        do 5 t''.
+                        do 5 t''.
+t. Defined.
+
+        Obligation 15.
+   (forall (str0 : String) (valid : nonterminal_names_listT)
+      (it : item CharType) (its : production CharType)
+      (str : String), H_prod_splitT' str0 valid None) ->
+   forall (str0 : String) (valid : nonterminal_names_listT)
+     (nonterminal_name : string)
+     (str : StringWithSplitState String
+              (split_stateT
+                 (include_nonterminal_name CharType nonterminal_name))),
+   let ret :=
+     DependentlyTyped.T_nonterminal_name_failure str0 valid nonterminal_name
+       str in
+   let arg :=
+     DependentlyTyped.T_productions_failure str0
+       (remove_nonterminal_name valid nonterminal_name)
+       (G nonterminal_name)
+       (lift_StringWithSplitState lift_lookup_nonterminal_name_state str) in
+   ~ Length str < Length str0 -> arg -> ret
+
+
+
+t. repeat t''.
+        apply remove_nonterminal_name_2 in H3.
+
+        exists x.
+        repeat t''.
+        destruct H3.
+        repeat t''.
+        split.
+        repeat t''.
+        repeat t''.
+        hnf in p0.
+        repeat t''.
+        hnf in p0.
+        SerachAbout
+
+
+        dependent destruction x.
+        repeat t''.
+        destruct f.
+        hnf in p0.
+        SearchAbout sub_names_listT.
+        pose (sub_names_listT_remove is_valid_nonterminal_name remove_nonterminal_name remove_name_1 _ _ _ H3).
+        SearchAbout sub_names_listT.
+        unique pose proof (
+ Defined.
         Obligation 16.
+
         t.
         { repeat t''.
           dependent destruction x.
